SStructTT/SStruct/Runtime/DropLemmas.lean
@@ -1,0 +1,169 @@
+import SStructTT.SStruct.Runtime.Step
+open ARS
+
+namespace SStruct.Erasure
+namespace Runtime
+
+variable {Srt : Type} [ord : SrtOrder Srt]
+
+lemma Drop.resolve {H1 H2 H3 H4 : Heap Srt} {m m'} :
+    Drop H3 m H4 -> H1 ⊢ m ▷ m' -> HMerge H1 H2 H3 ->
+    ∃ H0, HMerge H0 H2 H4 ∧ Contra H0 := by
+  intro dp rs mrg; induction rs generalizing H2 H3 H4
+  case var => cases dp; aesop
+  case lam => cases dp; aesop
+  case app mrg0 rsm rsn ihm ihn =>
+    cases dp; case app dp1 dp2 =>
+    have ⟨H1x, mrg1, mrg2⟩ := mrg.split mrg0.sym
+    have ⟨H2x, mrg3, ct3⟩ := ihm dp1 mrg2.sym
+    have ⟨H3x, mrg4, mrg5⟩ := mrg3.sym.split mrg1.sym
+    have ⟨H4x, mrg6, ct4⟩ := ihn dp2 mrg5.sym
+    have ⟨H5x, mrg7, mrg8⟩ := mrg6.sym.split mrg4.sym
+    existsi H5x; and_intros
+    . assumption
+    . apply mrg7.contra_image ct3 ct4
+  case tup mrg0 rsm rsn ihm ihn =>
+    cases dp; case tup dp1 dp2 =>
+    have ⟨H1x, mrg1, mrg2⟩ := mrg.split mrg0.sym
+    have ⟨H2x, mrg3, ct3⟩ := ihm dp1 mrg2.sym
+    have ⟨H3x, mrg4, mrg5⟩ := mrg3.sym.split mrg1.sym
+    have ⟨H4x, mrg6, ct4⟩ := ihn dp2 mrg5.sym
+    have ⟨H5x, mrg7, mrg8⟩ := mrg6.sym.split mrg4.sym
+    existsi H5x; and_intros
+    . assumption
+    . apply mrg7.contra_image ct3 ct4
+  case prj mrg0 rsm rsn ihm ihn =>
+    cases dp; case prj dp1 dp2 =>
+    have ⟨H1x, mrg1, mrg2⟩ := mrg.split mrg0.sym
+    have ⟨H2x, mrg3, ct3⟩ := ihm dp1 mrg2.sym
+    have ⟨H3x, mrg4, mrg5⟩ := mrg3.sym.split mrg1.sym
+    have ⟨H4x, mrg6, ct4⟩ := ihn dp2 mrg5.sym
+    have ⟨H5x, mrg7, mrg8⟩ := mrg6.sym.split mrg4.sym
+    existsi H5x; and_intros
+    . assumption
+    . apply mrg7.contra_image ct3 ct4
+  case tt => cases dp; aesop
+  case ff => cases dp; aesop
+  case ite mrg0 rsm1 rsn1 rsn2 ihm ihn1 ihn2 =>
+    cases dp; case ite dp1 dp2 =>
+    have ⟨H1x, mrg1, mrg2⟩ := mrg.split mrg0.sym
+    have ⟨H1x, mrg1, mrg2⟩ := mrg.split mrg0.sym
+    have ⟨H2x, mrg3, ct3⟩ := ihm dp1 mrg2.sym
+    have ⟨H3x, mrg4, mrg5⟩ := mrg3.sym.split mrg1.sym
+    have ⟨H4x, mrg6, ct4⟩ := ihn1 dp2 mrg5.sym
+    have ⟨H5x, mrg7, mrg8⟩ := mrg6.sym.split mrg4.sym
+    existsi H5x; and_intros
+    . assumption
+    . apply mrg7.contra_image ct3 ct4
+  case drop mrg0 rsm rsn ihm ihn =>
+    cases dp; case drop dp1 dp2 =>
+    have ⟨H1x, mrg1, mrg2⟩ := mrg.split mrg0.sym
+    have ⟨H2x, mrg3, ct3⟩ := ihm dp1 mrg2.sym
+    have ⟨H3x, mrg4, mrg5⟩ := mrg3.sym.split mrg1.sym
+    have ⟨H4x, mrg6, ct4⟩ := ihn dp2 mrg5.sym
+    have ⟨H5x, mrg7, mrg8⟩ := mrg6.sym.split mrg4.sym
+    existsi H5x; and_intros
+    . assumption
+    . apply mrg7.contra_image ct3 ct4
+  case null H1 _ => cases dp; aesop
+  case ptr lk1 rs ih =>
+    cases dp; case ptr lk2 dp =>
+    have ⟨e, mrg1⟩ := HLookup.collision mrg lk2 lk1
+    subst e; aesop
+
+lemma Resolve.drop_safeX {H1 H2 H3 : Heap Srt} {m m'} :
+    H1 ⊢ m ▷ m' -> HMerge H1 H2 H3 ->
+    ∃ H1' H3', Drop H3 m H3' ∧ HMerge H1' H2 H3' := by
+  intro rsm mrg; induction rsm generalizing H2 H3
+  case var H1 x ct =>
+    existsi H1, H3; and_intros
+    . constructor
+    . assumption
+  case lam ih =>
+    have ⟨Hx, Hy, dp, mrg⟩ := ih mrg
+    existsi Hx, Hy; and_intros
+    . constructor; assumption
+    . assumption
+  case app mrg1 rsm rsn ih1 ih2 =>
+    have ⟨Hx, mrg2, mrg3⟩ := mrg.split mrg1.sym
+    have ⟨Hy, H0, dp1, mrg4⟩ := ih1 mrg3.sym
+    have ⟨Hz, mrg5, mrg6⟩ := mrg4.sym.split mrg2.sym
+    have ⟨Ha, Hb, dp2, mrg7⟩ := ih2 mrg6.sym
+    have ⟨Hc, mrg8, mrg9⟩ := mrg7.sym.split mrg5.sym
+    existsi Hc, Hb; and_intros
+    . constructor
+      assumption
+      assumption
+    . assumption
+  case tup mrg1 rsm rsn ih1 ih2 =>
+    have ⟨Hx, mrg2, mrg3⟩ := mrg.split mrg1.sym
+    have ⟨Hy, H0, dp1, mrg4⟩ := ih1 mrg3.sym
+    have ⟨Hz, mrg5, mrg6⟩ := mrg4.sym.split mrg2.sym
+    have ⟨Ha, Hb, dp2, mrg7⟩ := ih2 mrg6.sym
+    have ⟨Hc, mrg8, mrg9⟩ := mrg7.sym.split mrg5.sym
+    existsi Hc, Hb; and_intros
+    . constructor
+      assumption
+      assumption
+    . assumption
+  case prj mrg1 rsm rsn ih1 ih2 =>
+    have ⟨Hx, mrg2, mrg3⟩ := mrg.split mrg1.sym
+    have ⟨Hy, H0, dp1, mrg4⟩ := ih1 mrg3.sym
+    have ⟨Hz, mrg5, mrg6⟩ := mrg4.sym.split mrg2.sym
+    have ⟨Ha, Hb, dp2, mrg7⟩ := ih2 mrg6.sym
+    have ⟨Hc, mrg8, mrg9⟩ := mrg7.sym.split mrg5.sym
+    existsi Hc, Hb; and_intros
+    . constructor
+      assumption
+      assumption
+    . assumption
+  case tt H1 _ =>
+    exists H1, H3; and_intros
+    . constructor
+    . assumption
+  case ff H1 _ =>
+    exists H1, H3; and_intros
+    . constructor
+    . assumption
+  case ite mrg1 rsm rsn1 rsn2 ih1 ih2 ih3 =>
+    have ⟨Hx, mrg2, mrg3⟩ := mrg.split mrg1.sym
+    have ⟨Hy, H0, dp1, mrg4⟩ := ih1 mrg3.sym
+    have ⟨Hz, mrg5, mrg6⟩ := mrg4.sym.split mrg2.sym
+    have ⟨Ha, Hb, dp2, mrg7⟩ := ih2 mrg6.sym
+    have ⟨Hc, mrg8, mrg9⟩ := mrg7.sym.split mrg5.sym
+    existsi Hc, Hb; and_intros
+    . constructor
+      assumption
+      assumption
+    . assumption
+  case drop mrg1 rsm rsn ih1 ih2 =>
+    have ⟨Hx, mrg2, mrg3⟩ := mrg.split mrg1.sym
+    have ⟨Hy, H0, dp1, mrg4⟩ := ih1 mrg3.sym
+    have ⟨Hz, mrg5, mrg6⟩ := mrg4.sym.split mrg2.sym
+    have ⟨Ha, Hb, dp2, mrg7⟩ := ih2 mrg6.sym
+    have ⟨Hc, mrg8, mrg9⟩ := mrg7.sym.split mrg5.sym
+    existsi Hc, Hb; and_intros
+    . constructor
+      assumption
+      assumption
+    . assumption
+  case ptr lk rs ih =>
+    have ⟨Hx, lk, mrg⟩ := lk.merge mrg
+    have ⟨Hy, Hz, dp, mrg⟩ := ih mrg
+    existsi Hy, Hz; and_intros
+    . constructor
+      assumption
+      assumption
+    . assumption
+  case null H1 _ =>
+    exists H1, H3; and_intros
+    . constructor
+    . assumption
+
+lemma Resolve.drop_safe {H1 : Heap Srt} {m m'} :
+    H1 ⊢ m ▷ m' -> ∃ H1', Drop H1 m H1' := by
+  intro rs
+  have ⟨H0, mrg, ct⟩ := HMerge.exists_self_contra H1
+  have ⟨H1', H3', dp, mrg⟩ := rs.drop_safeX mrg
+  have e := mrg.self_contra ct; subst e
+  existsi H1'; assumption
